update

Loda/Test/AstTest.lean
@@ -16,8 +16,8 @@ def δ₀ : Env.CircuitEnv := []
 -- --------------------------------------------------
 example : (Ast.Value.vInt 3) == (Ast.Value.vInt 3) := rfl
 example : (Ast.Value.vInt 3) != (Ast.Value.vInt 4) := rfl
-example : (Ast.Value.vStar) == (Ast.Value.vF 7 5) := rfl
-example : (Ast.Value.vF 7 4) == (Ast.Value.vStar) := rfl
+example : (Ast.Value.vStar) == (Ast.Value.vF 5) := rfl
+example : (Ast.Value.vF 4) == (Ast.Value.vStar) := rfl
 example : (Ast.Value.vBool true) != (Ast.Value.vBool false) := rfl
 
 -- --------------------------------------------------
@@ -31,53 +31,43 @@ example : Eval.evalRelOp Ast.RelOp.lt (Ast.Value.vBool true) (Ast.Value.vBool fa
 -- --------------------------------------------------
 -- eval on basic constants & var/let
 -- --------------------------------------------------
-example : Eval.eval σ₀ δ₀ (Ast.Expr.constInt 42) = some (Ast.Value.vInt 42) := by simp [Eval.eval]
-example : Eval.eval σ₀ δ₀ (Ast.Expr.constBool false) = some (Ast.Value.vBool false) := by simp [Eval.eval]
+example: Eval.EvalProp σ₀ δ₀ (.constInt 42) (.vInt 42) := Eval.EvalProp.ConstInt
+example: Eval.EvalProp σ₀ δ₀ (.constBool false) (.vBool false) := Eval.EvalProp.ConstBool
 
 def σ₁ := Env.updateVal σ₀ "y" (Ast.Value.vInt 99)
-example : Eval.eval σ₁ δ₀ (Ast.Expr.var "y") = some (Ast.Value.vInt 99) := by
-   simp [Eval.eval]
-   simp [σ₁]
-   unfold Env.updateVal
-   unfold Env.lookupVal
-   simp_all
+example: Eval.EvalProp σ₁ δ₀ (.var "y") (.vInt 99) := by
+  apply Eval.EvalProp.Var
+  simp [σ₁]
+  unfold Env.updateVal Env.lookupVal
+  simp_all
 
-example :
-  Eval.eval σ₀ δ₀ (Ast.Expr.letIn "z" (Ast.Expr.constInt 7) (Ast.Expr.intExpr (Ast.Expr.var "z") Ast.IntegerOp.mul (Ast.Expr.constInt 3)))
-  = some (Ast.Value.vInt 21) := by
-    simp [Eval.eval]
-    unfold Env.updateVal
-    unfold Env.lookupVal
-    unfold Eval.maximumRecursion
-    simp_all
+example: Eval.EvalProp σ₀ δ₀
+        (.letIn "z" (.constInt 7) (.intExpr (Ast.Expr.var "z") .mul (.constInt 3))) (.vInt 21) := by
+  apply Eval.EvalProp.Let
+  apply Eval.EvalProp.ConstInt
+  apply Eval.EvalProp.IntOp
+  apply Eval.EvalProp.Var
+  unfold Env.updateVal Env.lookupVal
+  simp_all
+  rfl
+  apply Eval.EvalProp.ConstInt
+  unfold Eval.evalIntegerOp
+  simp_all
 
-#eval Eval.eval σ₀ δ₀ (Ast.Expr.letIn "z" (Ast.Expr.constF 5 7) (Ast.Expr.fieldExpr (Ast.Expr.var "z") Ast.FieldOp.mul (Ast.Expr.constF 5 3)))
-#eval (HMul.hMul (7 : F 5) (3 : F 5))
+example: Eval.EvalProp σ₀ δ₀ (.binRel (.constInt 3) .le (.constInt 7)) (.vBool true) := by
+  apply Eval.EvalProp.Rel
+  apply Eval.EvalProp.ConstInt
+  apply Eval.EvalProp.ConstInt
+  unfold Eval.evalRelOp
+  simp_all
 
-example :
-  Eval.eval σ₀ δ₀ (Ast.Expr.letIn "z" (Ast.Expr.constF 5 7) (Ast.Expr.fieldExpr (Ast.Expr.var "z") Ast.FieldOp.mul (Ast.Expr.constF 5 3)))
-  = some (Ast.Value.vF 5 1) := by
-    simp [Eval.eval]
-    unfold Env.updateVal
-    unfold Env.lookupVal
-    simp_all
-    decide
-
-example :
-  Eval.eval σ₀ δ₀ (Ast.Expr.binRel (Ast.Expr.constInt 3) Ast.RelOp.le (Ast.Expr.constInt 7))
-  = some (Ast.Value.vBool true) := by
-    simp [Eval.eval]
-    unfold Eval.maximumRecursion
-    simp_all
-
-def pair := Ast.Expr.prodCons [Ast.Expr.constInt 2, Ast.Expr.constBool true]
-example :
-  Eval.eval σ₀ δ₀ pair
-  = some (Ast.Value.vProd [Ast.Value.vInt 2, Ast.Value.vBool true]) := by
-    unfold pair
-    simp [Eval.eval]
-    unfold Eval.maximumRecursion
-    simp_all
+def literalArr := Ast.Expr.arrCons (.constInt 5) (.arrCons [.constInt 0])
+example: Eval.EvalProp σ₀ δ₀ (.arrLen literalArr) (.vInt 2) := by
+  apply Eval.EvalProp.ArrLen
+  rw[literalArr]
+  apply Eval.EvalProp.ArrCons
+  apply Eval.EvalProp.ConstInt
+  apply Eval.EvalProp.ArrCons
 
 def literalArr := Ast.Expr.arrCons (Ast.Expr.constInt 5) (Ast.Expr.constInt 0) -- yields [5,0]
 example :
